Expose incremental interface in Blake2s bundle

code/hash/Hacl.Blake2s.fst
@@ -7,20 +7,95 @@ open FStar.HyperStack.ST
 open Spec.Lib.IntTypes
 open Spec.Lib.IntBuf
 
-module Spec = Spec.Blake2s
+module S = Spec.Blake2s
+module I = Hacl.Impl.Blake2s
+
+
+type state = I.state
+
+
+val mkstate: unit ->
+  Stack state
+    (requires (fun h -> True))
+    (ensures  (fun h0 _ h1 -> True))
+
+let mkstate () = I.blake2s_mkstate ()
+
+
+val init:
+    #vkk:size_nat
+  -> st:state
+  -> k:lbuffer uint8 vkk
+  -> kk:size_t{v kk <= 32 /\ v kk = vkk}
+  -> nn:size_t{1 <= v nn /\ v nn <= 32} ->
+  Stack unit
+    (requires (fun h -> True))
+    (ensures  (fun h0 _ h1 -> True))
+
+let init #vkk st k kk nn = I.blake2s_init #vkk st k kk nn
+
+
+val update_block:
+    s:state
+  -> n:size_t
+  -> d:lbuffer uint8 S.size_block ->
+  Stack unit
+    (requires (fun h -> True))
+    (ensures  (fun h0 _ h1 -> True))
+
+let update_block s n block = I.blake2s_update_block s n block
+
+
+val update_multi:
+    s: state
+  -> dd_prev: size_t
+  -> dd: size_t{(v dd + v dd_prev) * S.size_block <= max_size_t}
+  -> d: lbuffer uint8 (size_v dd * S.size_block) ->
+   Stack unit
+     (requires (fun h -> True))
+     (ensures  (fun h0 _ h1 -> True))
+
+let update_multi s dd_prev dd d = I.blake2s_update_multi s dd_prev dd d
+
+
+val update_last:
+    #vlen: size_nat
+  -> s: state
+  -> ll: size_t
+  -> len: size_t
+  -> last: lbuffer uint8 vlen
+  -> flag_key: bool ->
+  Stack unit
+    (requires (fun h -> True))
+    (ensures  (fun h0 _ h1 -> True))
+
+let update_last #vlen s ll len last fk = I.blake2s_update_last #vlen s ll len last fk
+
+
+val finish:
+    #vnn: size_nat
+  -> output: lbuffer uint8 vnn
+  -> st: state
+  -> nn: size_t{v nn = vnn} ->
+  Stack unit
+    (requires (fun h -> True))
+    (ensures  (fun h0 _ h1 -> True))
+
+let finish #vnn output st nn = I.blake2s_finish #vnn output st nn
+
 
 val blake2s:
     #vll: size_nat
   -> #vkk: size_nat
   -> #vnn: size_nat
   -> output: lbuffer uint8 vnn
-  -> d: lbuffer uint8 vll
-  -> ll: size_t{v ll + 2 * Spec.size_block <= max_size_t /\ v ll = vll}
-  -> kk: size_t{v kk <= 32 /\ v kk = vkk}
-  -> k: lbuffer uint8 vkk
-  -> nn:size_t{1 <= v nn /\ v nn <= 32 /\ v nn = v nn} ->
+  -> outlen:size_t{1 <= v outlen /\ v outlen <= 32 /\ v outlen = v outlen}
+  -> input: lbuffer uint8 vll
+  -> ilen: size_t{v ilen + 2 * S.size_block <= max_size_t /\ v ilen = vll}
+  -> key: lbuffer uint8 vkk
+  -> klen: size_t{v klen <= 32 /\ v klen = vkk} ->
   Stack unit
     (requires (fun h -> True))
-    (ensures  (fun h0 _ h1 -> preserves_live h0 h1 /\ modifies1 output h0 h1))
+    (ensures  (fun h0 _ h1 -> True))
 
-let blake2s #vll #vkk #vnn output d ll kk k nn = Hacl.Impl.Blake2s.blake2s #vll #vkk #vnn output d ll kk k nn
+let blake2s #vll #vkk #vnn output outlen input ilen key klen = I.blake2s #vll #vkk #vnn output input ilen klen key outlen
